The present section constrains the following binary columns: $\tinyBase$, $\tinyExponent$, $\oli{}$ and $\resVanishes$.
\begin{center}
\framebox{All constraints are written under the assumption that $\mulStamp_{i} \neq 0$.}
\end{center}
%\ob{TODO: maybe we should instead impose vanishing conditions when $\mulStamp_{i} = 0$. Probably not \dots{}}
We impose the following:
\begin{enumerate}
	\item \If $\iArgOneHi_{i} \neq 0$ \Then $\TINYBASE_{i} = 0$,
	\item \If $\iArgOneHi_{i} =    0$ \Then
	\begin{enumerate}
		\item \If $\iArgOneLo_{i} \cdot (1 - \iArgOneLo_{i}) \neq 0$ \Then $\TINYBASE_{i} = 0$;
		\item \If $\iArgOneLo_{i} \cdot (1 - \iArgOneLo_{i}) =    0$ \Then $\TINYBASE_{i} = 1$,
	\end{enumerate}
\end{enumerate}
similarly
\begin{enumerate}
	\item \If $\iArgTwoHi_{i} \neq 0$ \Then $\TINYEXPONENT_{i} = 0$;
	\item \If $\iArgTwoHi_{i} =    0$ \Then
	\begin{enumerate}
		\item \If $\iArgTwoLo_{i} \cdot (\iArgTwoLo_{i} - 1) \neq 0$ \Then $\TINYEXPONENT_{i} = 1$;
		\item \If $\iArgTwoLo_{i} \cdot (\iArgTwoLo_{i} - 1) =    0$ \Then $\TINYEXPONENT_{i} = 0$.
	\end{enumerate}
\end{enumerate}
further set
\begin{enumerate}
	\item \If $\iResHi_{i} \neq 0$ \Then $\RESVANISHES_{i} = 0$;
	\item \If $\iResHi_{i} =    0$ \Then
	\begin{enumerate}
		\item \If $\iResLo_{i} \neq 0$ \Then $\RESVANISHES_{i} = 0$;
		\item \If $\iResLo_{i} =    0$ \Then $\RESVANISHES_{i} = 1$.
	\end{enumerate}
\end{enumerate}
In other words
\[
	\left\{
	\begin{array}{lcl}
		\tinyBase = 1 & \iff & \iArgOne \in \{0,1\} \\
		\tinyExponent = 1 & \iff & \iArgTwo \in \{0,1\} \\
		\resVanishes = 1 & \iff & \iRes = 0 \\
	\end{array}
	\right.
\]
%\red{Note: we don't know at this point that $\iResHi$ and $\iResLo$ are indeed $\llarge$-byte integers. We thus \emph{can't} replace this by the simpler condition that $\resVanishes_{i} = 1$ \emph{iff} $\iResHi_{i} + \iResLo_{i} = 0$ as one might be tempted to do.}
Finally we set $\oli$ via $\oli = 1$ \emph{iff} \big($\tinyBase_{i} = 1$ \OR{} $\tinyExponent_{i} = 1$\big) i.e.
\[
	\oli_{i} =
	\tinyBase_{i} + \tinyExponent_{i} - \tinyBase_{i} \cdot \tinyExponent_{i}
\]