We now go on to consistency constraints proper.
\begin{description}
	\item[Setting the original storage value:]
		\If $\stoFirst_{i} = 1$ \Then
		we impose that
		\[
			\left\{ \begin{array}{lcl}
				\order{\stoOrigValueHi}_{i} & = & \order{\stoCurrValueHi}_{i} \\
				\order{\stoOrigValueLo}_{i} & = & \order{\stoCurrValueLo}_{i} \\
			\end{array} \right.
		\]
	\item[Resetting and resetting the original storage value:]
		\If $\order{\peekStorage}_{i} = 1$ \et $\stoFirst_{i} = 0$ \Then
		\begin{enumerate}
			\item \If $\order{\absTxNum}_{i} =    \order{\absTxNum}_{i - 1}$ \Then
				\[
					\left\{ \begin{array}{lcl}
						\order{\stoOrigValueHi}_{i} & = & \order{\stoOrigValueHi}_{i - 1} \\
						\order{\stoOrigValueLo}_{i} & = & \order{\stoOrigValueLo}_{i - 1} \\
					\end{array} \right.
				\]
			\item \If $\order{\absTxNum}_{i} \neq \order{\absTxNum}_{i - 1}$ \Then
				\[
					\left\{ \begin{array}{lcl}
						\order{\stoOrigValueHi}_{i} & = & \order{\stoCurrValueHi}_{i} \\
						\order{\stoOrigValueLo}_{i} & = & \order{\stoCurrValueLo}_{i} \\
					\end{array} \right.
				\]
		\end{enumerate}
	\item[Setting and resetting of storage values:]
		we impose that
		\begin{enumerate}
			\item \If $\stoFirst_{i} = 1$ \Then
				\begin{enumerate}
					\item \If $\order{\stoDeploymentNumber}_{i} \neq 0$ \Then
						\[
							\left\{ \begin{array}{lcl}
								\order{\stoCurrValueHi}_{i} & = & 0 \\
								\order{\stoCurrValueLo}_{i} & = & 0 \\
							\end{array} \right.
						\]
				\end{enumerate}
			\item \If $\order{\peekStorage}_{i} = 1$ \et $\stoFirst_{i} = 0$ \Then
				\begin{enumerate}
					\item \If $\order{\stoDeploymentNumber}_{i} \neq \order{\stoDeploymentNumber}_{i - 1}$ \Then
						\[
							\left\{ \begin{array}{lcl}
								\order{\stoCurrValueHi}_{i} & = & 0 \\
								\order{\stoCurrValueLo}_{i} & = & 0 \\
							\end{array} \right.
						\]
					\item \If $\order{\stoDeploymentNumber}_{i} = \order{\stoDeploymentNumber}_{i - 1}$ \Then
						\[
							\left\{ \begin{array}{lcl}
								\order{\stoCurrValueHi}_{i} & = & \order{\stoNextValueHi}_{i - 1} \\
								\order{\stoCurrValueLo}_{i} & = & \order{\stoNextValueLo}_{i - 1} \\
							\end{array} \right.
						\]
				\end{enumerate}
		\end{enumerate}
	\item[Setting and resetting of storage key warmth:]
		we impose that
		\begin{enumerate}
			\item \If $\stoFirst_{i} = 1$ \Then $\order{\stoWarmth}_{i} = 0$
			\item \If $\order{\peekStorage}_{i} = 1$ \et $\stoFirst_{i} = 0$ \Then
				\begin{enumerate}
					\item \If $\order{\absTxNum}_{i} =    \order{\absTxNum}_{i - 1}$ \Then $ \order{\stoWarmth}_{i} = \order{\stoWarmth\new}_{i - 1} $
					\item \If $\order{\absTxNum}_{i} \neq \order{\absTxNum}_{i - 1}$ \Then $ \order{\stoWarmth}_{i} = 0 $
				\end{enumerate}
		\end{enumerate}
	\item[Maintaining the final deployment number:]
		we impose that
			\item \If $\order{\peekStorage}_{i} = 1$ \et $\stoFirst_{i} = 0$ \Then $ \order{\stoDeploymentNumber^\infty}_{i} = \order{\stoDeploymentNumber^\infty}_{i - 1} $
\end{description}
