We impose the following constraints:
\begin{enumerate}
	\item $\hashInfoStamp_{0} = 0$
	\item \If $\hashInfoStamp_{i} = 0$ \Then 
		\[
			\left\{ \begin{array}{lcl}
				\hashInfoSize      _{i} & = & 0 \\
				\limb              _{i} & = & 0 \\
				\nBytes            _{i} & = & 0 \\
				\nBytesAcc         _{i} & = & 0 \\
			\end{array} \right.
		\]
	\item $\hashInfoStamp_{i + 1} \in \{ \hashInfoStamp_{i}, 1 + \hashInfoStamp_{i} \}$
	\item \If $\hashInfoStamp_{i} \neq \hashInfoStamp_{i - 1}$\footnote{In other words: \If $\hashInfoStamp_{i} = 1 + \hashInfoStamp_{i - 1}$} \Then
		\begin{enumerate}
			\item $\hashInfoSize_{i - 1} = \nBytesAcc_{i - 1}$
			\item $\nBytesAcc_{i} = \nBytes_{i}$
			\item $\index_{i} = 0$
		\end{enumerate}
	\item \If $\hashInfoStamp_{i} \neq 1 + \hashInfoStamp_{i - 1}$\footnote{In other words: \If $\hashInfoStamp_{i} = \hashInfoStamp_{i - 1}$} \Then
		\begin{enumerate}
			\item $\nBytesAcc_{i} = \nBytesAcc_{i - 1} + \nBytes_{i}$
			\item $\hashInfoSize_{i} = \hashInfoSize_{i - 1}$
			\item \If $\hashInfoStamp_{i} \neq 0$ \Then
				\begin{enumerate}
					\item $\nBytes_{i - 1} = \llarge$ \quad (\trash)
					\item $\index_{i} = 1 + \index_{i - 1}$
				\end{enumerate}
		\end{enumerate}
	\item $\hashInfoSize_{N} = \nBytesAcc_{N}$
\end{enumerate}
\saNote{} We \emph{could} add a ``nontriviality'' constraint such as ``\If $\hashInfoStamp_{i} \neq 0$ \Then $\hashInfoSize_{i} \neq 0$'', but there is no real point in doing so.
